Datatypes for metadata and spec validator v0.0

src/lowparse/LowParse.Spec.Parquet.fst
@@ -1,46 +1,735 @@
 module LowParse.Spec.Parquet
+
 module U32 = FStar.UInt32
+
 module U8 = FStar.UInt8
+
+module I8 = FStar.Int8
+
+module I16 = FStar.Int16
+
+module I32 = FStar.Int32
+
+module I64 = FStar.Int64
+
 module Seq = FStar.Seq
 
+module List = FStar.List
+
 open LowParse.Spec.Base
+
 open LowParse.Spec.RtoLDepPair
+
 open LowParse.Spec.RtoLPair
-open LowParse.Spec.Combinators // filter
-open LowParse.Spec.SeqBytes // "PAR1"
-open LowParse.Spec.BoundedInt // parse_u32_le
 
-assume val parse_footer_kind: parser_kind
-assume val footer_t: Type0
-assume val parse_footer: parser parse_footer_kind footer_t
+open LowParse.Spec.Combinators
 
-assume val parse_pages_kind: parser_kind
-assume val pages_t: (footer: footer_t) -> Type0
-assume val parse_pages: (footer: footer_t) -> parser parse_pages_kind (pages_t footer)
+open LowParse.Spec.SeqBytes
+
+open LowParse.Spec.BoundedInt
+
+open LowParse.Bytes
+
+open FStar.Real
+
+assume
+val parse_footer_kind:parser_kind
+
+assume
+val footer_t:Type0
+
+assume
+val parse_footer:parser parse_footer_kind footer_t
+
+assume
+val parse_pages_kind:parser_kind
+
+assume
+val pages_t (footer: footer_t) : Type0
+
+assume
+val parse_pages (footer: footer_t) : parser parse_pages_kind (pages_t footer)
 
 let is_PAR1 (s: Seq.lseq byte 4) : bool =
-    let v0 = Seq.index s 0 in
-    let v1 = Seq.index s 1 in
-    let v2 = Seq.index s 2 in
-    let v3 = Seq.index s 3 in
-    (U32.v (FStar.Char.u32_of_char 'P') = U8.v v0)
-    && (U32.v (FStar.Char.u32_of_char 'A') = U8.v v1)
-    && (U32.v (FStar.Char.u32_of_char 'R') = U8.v v2)
-    && (U32.v (FStar.Char.u32_of_char '1') = U8.v v3)
+  let v0 = Seq.index s 0 in
+  let v1 = Seq.index s 1 in
+  let v2 = Seq.index s 2 in
+  let v3 = Seq.index s 3 in
+  (U32.v (FStar.Char.u32_of_char 'P') = U8.v v0) && (U32.v (FStar.Char.u32_of_char 'A') = U8.v v1) &&
+  (U32.v (FStar.Char.u32_of_char 'R') = U8.v v2) &&
+  (U32.v (FStar.Char.u32_of_char '1') = U8.v v3)
+
+let parse_parquet =
+  parse_nondep_then_rtol (parse_filter (parse_seq_flbytes 4) is_PAR1)
+    (parse_dtuple2_rtol parse_u32_le
+        (fun len ->
+            (weaken (dtuple2_rtol_kind parse_seq_all_bytes_kind 0)
+                (parse_dtuple2_rtol (parse_fldata parse_footer (U32.v len))
+                    (fun footer ->
+                      // parse_pages footer
+                      (parse_seq_all_bytes))))))
 
 
-let parse_parquet  =
-  parse_nondep_then_rtol
-    (parse_filter (parse_seq_flbytes 4) is_PAR1)
-    (parse_dtuple2_rtol
-      parse_u32_le
-      fun len -> (
-        weaken (dtuple2_rtol_kind parse_seq_all_bytes_kind 0) (parse_dtuple2_rtol
-          (parse_fldata parse_footer (U32.v len))
-          fun footer -> (
-            parse_seq_all_bytes
-            // parse_pages footer
-          ))
-      )
-    )
-  
+
+// Enumerated Types
+
+type physical_type =
+  | BOOLEAN
+  | INT32
+  | INT64
+  | INT96
+  | FLOAT
+  | DOUBLE
+  | BYTE_ARRAY
+  | FIXED_LEN_BYTE_ARRAY
+
+type converted_type =
+  | DEPRECATED_UTF8
+  | DEPRECATED_MAP
+  | DEPRECATED_MAP_KEY_VALUE
+  | DEPRECATED_LIST
+  | DEPRECATED_ENUM
+  | DEPRECATED_DECIMAL
+  | DEPRECATED_DATE
+  | DEPRECATED_TIME_MILLIS
+  | DEPRECATED_TIME_MICROS
+  | DEPRECATED_TIMESTAMP_MILLIS
+  | DEPRECATED_TIMESTAMP_MICROS
+  | DEPRECATED_UINT_8
+  | DEPRECATED_UINT_16
+  | DEPRECATED_UINT_32
+  | DEPRECATED_UINT_64
+  | DEPRECATED_INT_8
+  | DEPRECATED_INT_16
+  | DEPRECATED_INT_32
+  | DEPRECATED_INT_64
+  | DEPRECATED_JSON
+  | DEPRECATED_BSON
+  | DEPRECATED_INTERVAL
+
+type field_repetition_type =
+  | REQUIRED
+  | OPTIONAL
+  | REPEATED
+
+type encoding =
+  | PLAIN
+  | PLAIN_DICTIONARY
+  | RLE
+  | BIT_PACKED
+  | DELTA_BINARY_PACKED
+  | DELTA_LENGTH_BYTE_ARRAY
+  | DELTA_BYTE_ARRAY
+  | RLE_DICTIONARY
+  | BYTE_STREAM_SPLIT
+
+type compression_codec =
+  | UNCOMPRESSED
+  | SNAPPY
+  | GZIP
+  | LZO
+  | BROTLI
+  | LZ4
+  | ZSTD
+  | LZ4_RAW
+
+type page_type =
+  | DATA_PAGE
+  | INDEX_PAGE
+  | DICTIONARY_PAGE
+  | DATA_PAGE_V2
+
+type boundary_order =
+  | UNORDERED
+  | ASCENDING
+  | DESCENDING
+
+type edge_interpolation_algorithm =
+  | SPHERICAL
+  | VINCENTY
+  | THOMAS
+  | ANDOYER
+  | KARNEY
+
+
+
+// Statistics and Metadata Structures
+
+type int64 = I64.t
+
+type int32 = I32.t
+
+type int16 = I16.t
+
+type int8 = I8.t
+
+type size_statistics = {
+  unencoded_byte_array_data_bytes:option int64;
+  repetition_level_histogram:option (list int64);
+  definition_level_histogram:option (list int64)
+}
+
+noeq
+type bounding_box = {
+  xmin:real;
+  xmax:real;
+  ymin:real;
+  ymax:real;
+  zmin:option real;
+  zmax:option real;
+  mmin:option real;
+  mmax:option real
+}
+
+noeq
+type geospatial_statistics = {
+  bbox:option bounding_box;
+  geospatial_types:option (list int32)
+}
+
+type statistics = {
+  max:option bytes;
+  min:option bytes;
+  null_count:option int64;
+  distinct_count:option int64;
+  max_value:option bytes;
+  min_value:option bytes;
+  is_max_value_exact:option bool;
+  is_min_value_exact:option bool
+}
+
+
+
+// Logical Types
+
+type string_type = unit
+
+type uuid_type = unit
+
+type map_type = unit
+
+type list_type = unit
+
+type enum_type = unit
+
+type date_type = unit
+
+type float16_type = unit
+
+type null_type = unit
+
+type json_type = unit
+
+type bson_type = unit
+
+type decimal_type = {
+  scale:int32;
+  precision:int32
+}
+
+type milli_seconds = unit
+
+type micro_seconds = unit
+
+type nano_seconds = unit
+
+type time_unit =
+  | MILLIS of milli_seconds
+  | MICROS of micro_seconds
+  | NANOS of nano_seconds
+
+type timestamp_type = {
+  isAdjustedToUTC:bool;
+  unit:time_unit
+}
+
+type time_type = {
+  isAdjustedToUTC:bool;
+  unit:time_unit
+}
+
+type int_type = {
+  bitWidth:int8;
+  isSigned:bool
+}
+
+type variant_type = { specification_version:option int8 }
+
+type geometry_type = { crs:option string }
+
+type geography_type = {
+  crs:option string;
+  algorithm:option edge_interpolation_algorithm
+}
+
+type logical_type =
+  | STRING of string_type
+  | MAP of map_type
+  | LIST of list_type
+  | ENUM of enum_type
+  | DECIMAL of decimal_type
+  | DATE of date_type
+  | TIME of time_type
+  | TIMESTAMP of timestamp_type
+  | INTEGER of int_type
+  | UNKNOWN of null_type
+  | JSON of json_type
+  | BSON of bson_type
+  | UUID of uuid_type
+  | FLOAT16 of float16_type
+  | VARIANT of variant_type
+  | GEOMETRY of geometry_type
+  | GEOGRAPHY of geography_type
+
+
+
+// Schema elements
+
+type schema_element = {
+  type_:option physical_type;
+  type_length:option int32;
+  repetition_type:option field_repetition_type;
+  name:string;
+  num_children:option int32;
+  converted_type:option converted_type;
+  scale:option int32;
+  precision:option int32;
+  field_id:option int32;
+  logical_type:option logical_type
+}
+
+
+
+// Page structures
+
+type data_page_header = {
+  num_values:int32;
+  encoding_:encoding;
+  definition_level_encoding:encoding;
+  repetition_level_encoding:encoding;
+  statistics:option statistics
+}
+
+type index_page_header = unit
+
+type dictionary_page_header = {
+  num_values:int32;
+  encoding:encoding;
+  is_sorted:option bool
+}
+
+type data_page_header_v2 = {
+  num_values:int32;
+  num_nulls:int32;
+  num_rows:int32;
+  encoding:encoding;
+  definition_levels_byte_length:int32;
+  repetition_levels_byte_length:int32;
+  is_compressed:option bool;
+  statistics:option statistics
+}
+
+
+
+// Bloom Filters
+
+type split_block_algorithm = unit
+
+type bloom_filter_algorithm = | BLOCK of split_block_algorithm
+
+type xx_hash = unit
+
+type bloom_filter_hash = | XXHASH of xx_hash
+
+type uncompressed = unit
+
+type bloom_filter_compression = | UN_COMPRESSED of uncompressed
+
+type bloom_filter_header = {
+  numBytes:int32;
+  algorithm:bloom_filter_algorithm;
+  hash:bloom_filter_hash;
+  compression:bloom_filter_compression
+}
+
+
+
+// Column chunks
+
+// type page_header_variants =
+//   | DATA_PAGE_HEADER of data_page_header
+//   | INDEX_PAGE_HEADER of index_page_header
+//   | DICTIONARY_PAGE_HEADER of dictionary_page_header
+//   | DATA_PAGE_HEADER_V2 of data_page_header_v2
+
+type page_header = {
+  ptype: page_type;
+  uncompressed_page_size:int32;
+  compressed_page_size:int32;
+  crc:option int32;
+  data_page_header: option data_page_header;
+  index_page_header: option index_page_header;
+  dictionary_page_header: option dictionary_page_header;
+  data_page_header_v2: option data_page_header_v2
+  // header:page_header_variants // sum type instead of "tagged union"
+}
+
+
+
+type key_value = {
+  key:string;
+  value:option string
+}
+
+type sorting_column = {
+  column_idx:int32;
+  descending:bool;
+  nulls_first:bool
+}
+
+type page_encoding_stats = {
+  page_type:page_type;
+  encoding:encoding;
+  count:int32
+}
+
+noeq
+type column_meta_data = {
+  physical_type:physical_type;
+  encodings:list encoding;
+  path_in_schema:list string;
+  codec:compression_codec;
+  num_values:int64;
+  total_uncompressed_size:int64;
+  total_compressed_size:int64;
+  key_value_metadata:option (list key_value);
+  data_page_offset:int64;
+  index_page_offset:option int64;
+  dictionary_page_offset:option int64;
+  statistics:option statistics;
+  encoding_stats:option (list page_encoding_stats);
+  bloom_filter_offset:option int64;
+  bloom_filter_length:option int32;
+  size_statistics:option size_statistics;
+  geospatial_statistics:option geospatial_statistics
+}
+
+type encryption_with_footer_key = unit
+
+type encryption_with_column_key = {
+  path_in_schema:list string;
+  key_metadata:option string
+}
+
+type column_crypto_meta_data =
+  | ENCRYPTION_WITH_FOOTER_KEY of encryption_with_footer_key
+  | ENCRYPTION_WITH_COLUMN_KEY of encryption_with_column_key
+
+noeq
+type column_chunk = {
+  file_path:option string;
+  file_offset:int64;
+  meta_data:option column_meta_data; // can be required for featherweight parquet
+  offset_index_offset:option int64;
+  offset_index_length:option int32;
+  column_index_offset:option int64;
+  column_index_length:option int32;
+  crypto_metadata:option column_crypto_meta_data;
+  encrypted_column_metadata:option string
+}
+
+noeq
+type row_group = {
+  columns:list column_chunk;
+  total_byte_size:int64;
+  num_rows:int64;
+  sorting_columns:option (list sorting_column);
+  file_offset:option int64;
+  total_compressed_size:option int64;
+  ordinal:option int16
+}
+
+type type_defined_order = unit
+
+type column_order = | TYPE_ORDER of type_defined_order
+
+type page_location = {
+  offset:int64;
+  compressed_page_size:int32;
+  first_row_index:int64
+}
+
+type offset_index = {
+  page_locations:list page_location;
+  unencoded_byte_array_data_bytes:option (list int64)
+}
+
+type column_index = {
+  null_pages:list bool;
+  min_values:list string;
+  max_values:list string;
+  boundary_order:boundary_order;
+  null_counts:option (list int64);
+  repetition_level_histograms:option (list int64);
+  definition_level_histograms:option (list int64)
+}
+
+type aes_gcm_v1 = {
+  aad_prefix:option string;
+  aad_file_unique:option string;
+  supply_aad_prefix:option bool
+}
+
+type aes_gcm_ctr_v1 = {
+  aad_prefix:option string;
+  aad_file_unique:option string;
+  supply_aad_prefix:option bool
+}
+
+type encryption_algorithm =
+  | AES_GCM_V1 of aes_gcm_v1
+  | AES_GCM_CTR_V1 of aes_gcm_ctr_v1
+
+noeq
+type file_meta_data = {
+  version:int32;
+  schema:list schema_element;
+  num_rows:int64;
+  row_groups:list row_group;
+  key_value_metadata:option (list key_value);
+  created_by:option string;
+  column_orders:option (list column_order);
+  encryption_algorithm:option encryption_algorithm;
+  footer_signing_key_metadata:option string
+}
+
+type file_crypto_meta_data = {
+  encryption_algorithm:encryption_algorithm;
+  key_metadata:option string
+}
+
+
+
+(* Another separate pass to check offset_index and column_index *)
+(* They don't overlap with the footer metadata *)
+
+(*
+  File: A HDFS file that must include the metadata for the file. It does not need to actually contain the data.
+
+  Row group: A logical horizontal partitioning of the data into rows. There is no physical structure that is guaranteed for a row group. A row group consists of a column chunk for each column in the dataset.
+
+  Column chunk: A chunk of the data for a particular column. They live in a particular row group and are guaranteed to be contiguous in the file.
+
+  Page: Column chunks are divided up into pages. A page is conceptually an indivisible unit (in terms of compression and encoding). There can be multiple page types which are interleaved in a column chunk.
+
+  Hierarchically, a file consists of one or more row groups. A row group contains exactly one column chunk per column. Column chunks contain one or more pages.
+
+  1. Check offset_index and column_index (They don't overlap with the footer metadata)
+  2. Check the correctness of all the offsets and sizes (disjointness among all pages)
+  3. Check the order (page locations per column chunk)
+  4. Check that the sizes of children should add up to the same size of the parents
+  5. Check the list schema_element is of the same tree structure of the rowgroup's list column_chunk
+  6. Check the physical types of column_meta_data against the schema
+  7. Check the actual data value against the phycial/logical type (will be slow, except for e.g., ints)
+  8. Statistics can be checked, but only for optimization (to skip pages efficiently)
+ *)
+// val validate_file_metat_data (fmd: file_meta_data) : bool
+
+// let validate_file_metat_data (fmd: file_meta_data) : bool = true
+
+(** Helpers ----------------------------------------------------------- *)
+
+let rec zip (#a #b: Type0) (xs: list a) (ys: list b {List.length ys == List.length xs})
+    : Tot (list (a & b)) =
+  match xs, ys with
+  | [], [] -> []
+  | x :: xs', y :: ys' -> (x, y) :: (zip xs' ys')
+
+
+
+(* A byte‑range in the file *)
+
+type range = {
+  start:int64;
+  len:int32
+}
+
+let range_end (r: range) : int = I64.v r.start + I32.v r.len
+
+
+
+(* Two ranges are disjoint iff they don’t overlap *)
+
+let disjoint (r1 r2: range) : Tot bool =
+  let end1 = range_end r1 in
+  let end2 = range_end r2 in
+  (I64.v r1.start >= end2) || (I64.v r2.start >= end1)
+
+
+
+(* Check if a list of ranges are disjoint *)
+
+let rec ranges_disjoint (rs: list range) : Tot bool =
+  match rs with
+  | [] | [_] -> true
+  | x :: xs -> List.Tot.for_all (disjoint x) xs && ranges_disjoint xs
+
+
+
+(* Build a range from optional offset/length *)
+
+let range_of_offsets (off: option int64) (len: option int32) : option range =
+  match off, len with
+  | Some o, Some l -> Some ({ start = o; len = l })
+  | _ -> None
+
+
+
+// (* Sum a list<int32> into int64 safely *)
+// let sum_i32 (xs:list int32) : Tot int64 =
+//   List.Tot.fold_left (fun acc x -> acc + int64 (v x)) 0L xs
+
+let rec offsets_are_ordered (prev: page_location) (locs: list page_location)
+    : Tot bool (decreases locs) =
+  match locs with
+  | [] -> true
+  | loc :: rest -> I64.v loc.offset >= I64.v prev.offset && offsets_are_ordered loc rest
+
+
+
+(** Validation of a single column‑chunk ------------------------------ *)
+
+val validate_column_chunk: column_chunk -> int64 -> option offset_index -> Tot bool
+
+let validate_column_chunk cc footer_start oi =
+  let idx_ranges:(* 1. index ranges must be disjoint and not overlap with footer *)
+  list range =
+    let off_idx = range_of_offsets cc.offset_index_offset cc.offset_index_length in
+    let col_idx = range_of_offsets cc.column_index_offset cc.column_index_length in
+    match off_idx, col_idx with
+    | Some r1, Some r2 -> [r1; r2]
+    | Some r, None | None, Some r -> [r]
+    | None, None -> []
+  in
+  let idx_ok =
+    ranges_disjoint idx_ranges &&
+    List.Tot.for_all (fun r -> range_end r <= I64.v footer_start) idx_ranges
+  in
+  let pages_ok =
+    (* 2. page‑level checks when we have an OffsetIndex *)
+    match oi with
+    | None -> true
+    | Some oi' ->
+      let locs = oi'.page_locations in
+      let ordered =
+        (* ordered by offset and disjoint *)
+        match locs with
+        | [] -> true
+        | first :: rest -> offsets_are_ordered first rest
+      in
+      let disj =
+        let pl_ranges =
+          List.Tot.map (fun pl -> { start = pl.offset; len = pl.compressed_page_size }) locs
+        in
+        ranges_disjoint pl_ranges
+      in
+      let col_size_ok =
+        (* compressed size matches meta *)
+        match cc.meta_data with
+        | None -> true
+        | Some md ->
+          let s = List.Tot.fold_left (fun acc pl -> acc + I32.v pl.compressed_page_size) 0 locs in
+          s = I64.v md.total_compressed_size
+      in
+      ordered && disj && col_size_ok
+  in
+  idx_ok && pages_ok
+
+
+
+(** Column order vs schema order ------------------------------------- *)
+
+(** Row‑group validation --------------------------------------------- *)
+
+let offset_of_column_chunk (cmd: column_meta_data) : int64 =
+  match cmd.dictionary_page_offset with
+  | Some off -> off
+  | None ->
+    match cmd.index_page_offset with
+    | Some off -> if I64.v off < I64.v cmd.data_page_offset then off else cmd.data_page_offset
+    | None -> cmd.data_page_offset
+
+let rec columns_are_contiguous (prev: column_chunk) (cols: list column_chunk)
+    : Tot bool (decreases cols) =
+  match cols with
+  | [] -> true
+  | cc :: rest ->
+    match prev.meta_data, cc.meta_data with
+    | Some (prev_md: column_meta_data), Some cc_md ->
+      let prev_offset = I64.v (offset_of_column_chunk prev_md) in
+      let cc_offset = I64.v (offset_of_column_chunk cc_md) in
+      let prev_size = I64.v prev_md.total_compressed_size in
+      prev_offset + prev_size = cc_offset && columns_are_contiguous cc rest
+    | _ ->
+      // if metadata is missing, we can't check contiguity
+      true
+
+val validate_row_group: row_group -> int64 -> list (option offset_index) -> Tot bool
+
+let validate_row_group rg footer_start offset_indices =
+  let col_sizes:(* sum of col sizes equals row‑group size (when available) *)
+  list (option int64) =
+    List.Tot.map (fun cc ->
+          match cc.meta_data with
+          | None -> None
+          | Some md -> Some md.total_compressed_size)
+      rg.columns
+  in
+  let rg_size_ok =
+    match rg.total_compressed_size with
+    | None -> true
+    | Some sz ->
+      let total_size =
+        List.Tot.fold_left (fun acc sz_opt ->
+              match acc, sz_opt with
+              | Some acc_sz, Some sz -> Some (acc_sz + I64.v sz)
+              | _, _ -> None)
+          (Some 0)
+          col_sizes
+      in
+      match total_size with
+      | None -> true
+      | Some total_sz -> total_sz = I64.v sz
+  in
+  let contiguous_ok =
+    (* cols should be contiguous *)
+    match rg.columns with
+    | [] -> true
+    | first :: rest -> columns_are_contiguous first rest
+  in
+  let cols_ok =
+    (* each column chunk passes *)
+    if List.length offset_indices = List.length rg.columns
+    then
+      List.Tot.for_all (fun (cc, oi) -> validate_column_chunk cc footer_start oi)
+        (zip rg.columns offset_indices)
+    else false
+  in
+  rg_size_ok && contiguous_ok && cols_ok
+
+
+
+(** Top‑level file metadata validation ------------------------------- *)
+
+val validate_file_metat_data: file_meta_data -> int64 -> list (list (option offset_index))
+  -> Tot bool
+
+let validate_file_metat_data fmd footer_start group_offset_indices =
+  if List.length group_offset_indices = List.length fmd.row_groups
+  then
+    List.Tot.for_all (fun (rg, offset_indices) ->
+          if List.length offset_indices = List.length rg.columns
+          then validate_row_group rg footer_start offset_indices
+          else false)
+      (zip fmd.row_groups group_offset_indices)
+  else false
